theories/L/AbstractMachines/FlatPro/Programs.v
@@ -1,24 +1,8 @@
-From Undecidability.L Require Import Prelim.MoreBase L.
+From Undecidability.L Require Import Prelim.MoreBase L AbstractMachines.LargestVar.
+Require Import Lia.
+Require Export Undecidability.L.AbstractMachines.FlatPro.ProgramsDef.
 
 (** * Abstract L machines *)
-(** ** Encoding Terms as Programs *)
-
-Inductive Tok := varT (n :nat) | appT | lamT | retT.
-Notation Pro := (list Tok) (only parsing).
-
-Instance Tok_eq_dec : eq_dec Tok.
-repeat intro. hnf. repeat decide equality.
-Qed.
-
-Fixpoint compile (s: L.term) : Pro :=
-  match s with
-    var x => [varT x]
-  | app s t => compile s ++ compile t ++ [appT]
-  | lam s => lamT :: compile s ++ [retT]
-  end.
-
-Inductive reprP : Pro -> term -> Prop :=
-  reprPC s : reprP (compile s) (lam s).
 
 (** *** Program size *)
 
@@ -49,6 +33,18 @@ Proof.
   all:autorewrite with list. all:cbn. all:try omega.
 Qed.
 
+
+Lemma le_length_sizeP P :
+  length P <= sizeP P.
+Proof.
+  unfold sizeP. induction P as [|[]];cbn in *;try Lia.lia.
+Qed.
+
+
+Lemma length_compile_leq s : |compile s| <= 2*size s.
+Proof.
+  induction s;cbn. all:autorewrite with list;cbn. all:nia.
+Qed.
 
 (** *** Programm Decomposition *)
 
@@ -113,22 +109,23 @@ Qed.
 
 (** *** Injectivity of Programm Encoding *)
 
-Fixpoint decompile l P A : option (list term) :=
+(** returning the internal state as inr allows for stronger results w.r.t. decompiling initial segments*)
+Fixpoint decompile l P A {struct P}: (list term) + (nat * Pro * list term) :=
   match P with
     retT::P => match l with
-                0 => None
+                0 => inr (l,retT::P,A)
               | S l => match A with
                         s::A => decompile l P (lam s::A)
-                      | [] => None
+                      | [] => inr (S l, retT::P, A)
                       end
               end
   | varT n::P => decompile l P (var n::A)
   | lamT::P =>  decompile (S l) P A
   | appT::P => match A with
                t::s::A => decompile l P (app s t::A)
-             | _ => None
+             | _ => inr (l, appT::P, A)
               end
-  | [] => Some A
+  | [] => inl A
   end.
 
 Lemma decompile_correct' l s P A:
@@ -140,6 +137,29 @@ Proof.
   -autorewrite with list. rewrite IHs. reflexivity.
 Qed.
 
+
+Lemma decompile_correct l s:
+  decompile l (compile s) [] = inl [s].
+Proof.
+  specialize (decompile_correct' l s [] []) as H. autorewrite with list in H. rewrite H. easy.
+Qed.
+
+(** We can not show a lemma that if decompile produces a term, the inout was a compilation as decompile itself sometimes decompiles incorrect programs if the lamTs are at wrong positions*)
+Lemma decompile_resSize l P A B:
+  decompile l P A = inl B -> sumn (map size B) <= sumn (map size A) + sumn (map sizeT P).
+Proof.
+  induction P as [ |[] P] in l,A|-*.
+  -cbn. intros [= ->]. nia.
+  -cbn. intros ->%IHP. cbn. nia.
+  -destruct A as [ | ? []]. 1,2:easy.
+   intros ->%IHP. cbn. nia.
+  -cbn.  intros ->%IHP. nia.
+  -destruct l. easy.
+   destruct A as []. 1:easy.
+   intros ->%IHP. cbn. nia.
+   all:cbn.
+Qed.
+
 Lemma compile_inj s s' :
   compile s = compile s' -> s = s'.
 Proof.
@@ -147,4 +167,60 @@ Proof.
   specialize (@decompile_correct' 0 s [] []) as H1.
   specialize (@decompile_correct' 0 s' [] []) as H2.
   rewrite eq in H1. rewrite H1 in H2. now inv H2.
+Qed.
+
+Lemma compile_neq_nil s:
+  compile s <> [].
+Proof.
+  edestruct (compile s) eqn:eq. 2:easy.
+  specialize decompile_correct' with (l:=0) (s:=s) (P:=[]) (A:=[]).
+  rewrite eq.
+  cbn. easy.
+Qed.
+
+Lemma compile_inj_retT s s' P P':
+  compile s ++ retT::P = compile s' ++ retT::P' -> s = s' /\ P = P'.
+Proof.
+  intros eq.
+  specialize (@decompile_correct' 0 s (retT::P) []) as H1.
+  specialize (@decompile_correct' 0 s' (retT::P') []) as H2.
+  rewrite eq in H1. rewrite H1 in H2.
+  now inv H2.
+Qed.
+
+Definition Tok_eqb (t t' : Tok) :=
+  match t,t' with
+    varT n, varT n' => Nat.eqb n n'
+  | retT,retT => true
+  | lamT, lamT => true
+  | appT, appT => true
+  | _,_ => false
+  end.
+
+Lemma Tok_eqb_spec t t' : reflect (t = t') (Tok_eqb t t').
+Proof.
+  destruct t,t'. all:cbn. destruct (Nat.eqb_spec n n0);[subst|].
+  all:try left;eauto.
+  all:right;congruence.
+Qed.
+
+Definition largestVarT t :=
+  match t with
+    varT n => n
+  | _ => 0
+  end.
+
+
+Definition largestVarP P := maxl (map largestVarT P).
+
+Lemma largestVar_compile s :
+  largestVarP (compile s) = largestVar s.
+Proof.
+  unfold largestVarP in *. 
+  induction s;cbn.
+  -Lia.lia.
+  -autorewrite with list. rewrite ! maxl_app.
+   rewrite IHs1,IHs2. cbn. Lia.lia.
+  -autorewrite with list. rewrite ! maxl_app.
+   rewrite IHs. cbn. Lia.lia.
 Qed.
