theories/L/Datatypes/Lists.v
@@ -1,5 +1,7 @@
 From Undecidability.L.Tactics Require Import LTactics GenEncode.
+From Undecidability.L Require Import Functions.EqBool.
 From Undecidability.L.Datatypes Require Import LBool LNat LOptions LProd.
+From Undecidability.L Require Import UpToC.
 Require Export List PslBase.Lists.Filter Datatypes.
 
 (** ** Encoding of lists *)
@@ -7,13 +9,13 @@ Require Export List PslBase.Lists.Filter Datatypes.
 Section Fix_X.
   Variable (X:Type).
   Context {intX : registered X}.
-
+  Import GenEncode.
   Run TemplateProgram (tmGenEncode "list_enc" (list X)).  
   Hint Resolve list_enc_correct : Lrewrite.
   
   (* now we must register the non-constant constructors*)
   
-  Global Instance termT_cons : computableTime (@cons X) (fun a aT => (1,fun A AT => (1,tt))).
+  Global Instance termT_cons : computableTime' (@cons X) (fun a aT => (1,fun A AT => (1,tt))).
   Proof using intX.
     extract constructor.
     solverec.
@@ -25,13 +27,13 @@ Section Fix_X.
   (* Qed. *)
   
 
-  Global Instance termT_append : computableTime (@List.app X) (fun A _ => (5,fun B _ => (length A * 16 +4,tt))).
-  Proof  using intX.
+  Global Instance termT_append : computableTime' (@List.app X) (fun A _ => (5,fun B _ => (length A * 16 +4,tt))).
+  Proof using intX.
     extract.
     solverec.
   Qed.
 
-  Global Instance term_filter: computableTime (@filter X) (fun p pT => (1,fun l _ => (fold_right (fun x res => 16 + res + fst (pT x tt)) 8 l ,tt))).
+  Global Instance term_filter: computableTime' (@filter X) (fun p pT => (1,fun l _ => (fold_right (fun x res => 16 + res + fst (pT x tt)) 8 l ,tt))).
   Proof using intX.
     change (filter (A:=X)) with ((fun (f : X -> bool) =>
                                     fix filter (l : list X) : list X := match l with
@@ -48,7 +50,7 @@ Section Fix_X.
     computable using t.
   Defined.
 
-  Global Instance term_nth : computableTime (@nth X) (fun n _ => (5,fun l lT => (1,fun d _ => (n*20+9,tt)))). 
+  Global Instance term_nth : computableTime' (@nth X) (fun n _ => (5,fun l lT => (1,fun d _ => (n*20+9,tt)))). 
   Proof using intX.
     extract.
     solverec.
@@ -75,7 +77,7 @@ Section Fix_X.
       *constructor. tauto.
   Qed.
 
-  Global Instance term_inb: computableTime inb (fun eq eqT => (5,fun x _ => (1,fun l _ =>
+  Global Instance term_inb: computableTime' inb (fun eq eqT => (5,fun x _ => (1,fun l _ =>
                                         (fold_right (fun x' res => callTime2 eqT x' x
                                                                 + res + 17) 4 l ,tt)))).
   Proof.
@@ -116,12 +118,31 @@ Section Fix_X.
 End Fix_X.
 
 Hint Resolve list_enc_correct : Lrewrite.
+
+Fixpoint map_time {X} (fT:X -> nat) xs :=
+  match xs with
+    [] => 8
+  | x :: xs => fT x + map_time fT xs + 12
+  end.
   
-Instance term_map (X Y:Type) (Hx : registered X) (Hy:registered Y): computableTime (@map X Y) (fun f fT => (1,fun l _ => (fold_right (fun x res => fst (fT x tt) + res + 12) 8 l,tt))).
+Instance term_map (X Y:Type) (Hx : registered X) (Hy:registered Y): computableTime' (@map X Y) (fun _ fT => (1,fun l _ => (map_time (fun x => fst (fT x tt)) l,tt))).
 Proof.
   extract.
   solverec.
 Defined.
+
+Lemma map_time_const {X} c (xs:list X):
+  map_time (fun _ => c) xs = length xs * (c + 12) + 8.
+Proof.
+  induction xs;cbn. all:lia.
+Qed.
+
+Lemma mapTime_upTo X (t__f : X -> nat):
+  map_time t__f <=c (fun l => length l + sumn (map t__f l) + 1 ).
+Proof.
+  unfold map_time. exists 12.
+  induction x;cbn - [plus mult]. all: nia.
+Qed.
 
 Instance term_map_noTime (X Y:Type) (Hx : registered X) (Hy:registered Y): computable (@map X Y).
 Proof.
@@ -129,22 +150,22 @@ Proof.
 Defined.
 
 
-Instance termT_nth_error (X:Type) (Hx : registered X): computableTime (@nth_error X) (fun A _ => (5,fun n _ => (min n (length A)*15 + 10,tt))).
+Instance termT_nth_error (X:Type) (Hx : registered X): computableTime' (@nth_error X) (fun A _ => (5,fun n _ => (min n (length A)*15 + 10,tt))).
 Proof.
   extract. solverec.
 Qed.
 
-Instance termT_length X `{registered X} : computableTime (@length X) (fun A _ => ((length A)*11+8,tt)).
+Instance termT_length X `{registered X} : computableTime' (@length X) (fun A _ => ((length A)*11+8,tt)).
 extract. solverec.
 Qed.
 
-Instance termT_rev_append X `{registered X}: computableTime (@rev_append X) (fun l _ => (5,fun res _ => (length l*13+4,tt))).
+Instance termT_rev_append X `{registered X}: computableTime' (@rev_append X) (fun l _ => (5,fun res _ => (length l*13+4,tt))).
 extract.
 recRel_prettify.
 solverec.
 Qed.
 
-Instance termT_rev X `{registered X}: computableTime (@rev X) (fun l _ => (length l*13+10,tt)).
+Instance termT_rev X `{registered X}: computableTime' (@rev X) (fun l _ => (length l*13+10,tt)).
 eapply computableTimeExt with (x:= fun l => rev_append l []).
 {intro. rewrite rev_alt. reflexivity. }
 extract. solverec.
@@ -187,7 +208,7 @@ Section int.
     | _,_ => 9
     end.
   
-  Global Instance term_list_eqb : computableTime (list_eqb (X:=X))
+  Global Instance term_list_eqb : computableTime' (list_eqb (X:=X))
                                                    (fun _ eqbT => (1,(fun A _ => (5,fun B _ => (list_eqbTime eqbT A B,tt))))).
   Proof.
     extract.
@@ -204,9 +225,77 @@ Section int.
      {cbn. intuition. }
      cbn - [callTime2]. setoid_rewrite IHA.
      rewrite H'. ring_simplify. intuition.
-  Qed.             
+  Qed.
+
+  
+  Lemma list_eqbTime_bound_r (eqbT : timeComplexity (X -> X -> bool)) (A B : list X) f:
+    (forall (x y:X), callTime2 eqbT x y <= f y) ->
+    list_eqbTime eqbT A B <= sumn (map f B) + 9 + length B * 22.
+  Proof.
+    intros H.
+    induction A in B|-*;unfold list_eqbTime;fold list_eqbTime. now Lia.lia.
+    destruct B.
+    -cbn. Lia.lia.
+    -rewrite H,IHA. cbn [length map sumn]. Lia.lia.
+  Qed.
+
+  Global Instance eqbList f `{eqbClass (X:=X) f}:
+    eqbClass (list_eqb f).
+  Proof.
+    intros ? ?. eapply list_eqb_spec. all:eauto using eqb_spec.
+  Qed.
+  Import EqBool.
+  Global Instance eqbComp_List `{eqbCompT X (R:=HX)}:
+    eqbCompT (list X).
+  Proof.
+    evar (c:nat). exists c. unfold list_eqb. 
+    unfold enc;cbn.
+    change (eqb0) with (eqb (X:=X)).
+    extract. unfold eqb,eqbTime. fold @enc.
+    recRel_prettify2. easy.
+    [c]:exact (c__eqbComp X + 6).
+    all:unfold c. all:cbn iota beta delta [list_enc].
+    all:  change ((match HX with
+                   | @mk_registered _ enc _ _ => enc
+                   end)) with (enc (X:=X)).
+    all:cbn [size]. all: nia.
+  Qed.
   
 End int.
+
+
+Instance term_length X {H:registered X}:
+  computableTime' (@length X) (fun t _ => (length t * 11 + 8,tt)).  
+extract. solverec.
+Proof.
+Qed.
+
+
+Fixpoint forallb_time {X} (fT:X -> nat) xs :=
+  match xs with
+    [] => 8
+  | x :: xs => fT x + forallb_time fT xs + 15
+  end.
+
+Lemma forallb_time_eq X f (l:list X):
+  forallb_time f l = sumn (map f l) + length l * 15 + 8.
+Proof.
+  induction l;cbn;nia.
+Qed.
+
+Lemma forallb_time_const X c (l:list X):
+  forallb_time (fun _ =>  c) l = length l * (c+15) + 8.
+Proof.
+  induction l;cbn;nia.
+Qed.
+
+Instance term_forallb X {HX:registered X}:
+  computableTime' (@forallb X) (fun f t__f => (1,fun l _ => (forallb_time (fun x => fst (t__f x tt)) l,tt))).
+Proof.
+  extract.
+  solverec.
+Qed.
+
 
 Section list_prod.
 
@@ -226,4 +315,107 @@ Section list_prod.
   Qed.
 
 End list_prod.
+
+
+Lemma size_list X `{registered X} (l:list X):
+  size (enc l) = sumn (map (fun x => size (enc x) + 5) l)+ 4.
+Proof.
+  change (enc l) with (list_enc l).
+  induction l.
+  -easy.
+  -cbn [list_enc map sumn size].
+   change ((match H with
+            | @mk_registered _ enc _ _ => enc
+            end a)) with (enc a). solverec. 
+Qed.
+
+Lemma size_list_cons (X : Type) (H : registered X) x (l : list X):
+  size (enc (x::l)) = size (enc x) + size (enc l) + 5.
+Proof.
+  rewrite !size_list. cbn. lia.
+Qed.
+
+Lemma size_list_enc_r {X} `{registered X} (l:list X):
+  length l <= size (enc l).
+Proof.
+  rewrite size_list. induction l;cbn. all:lia.
+Qed.
+
+Instance term_repeat A `{registered A}: computableTime' (@repeat A) (fun _ _ => (5, fun n _ => (n * 12 + 4,tt))).
+Proof.
+  extract. solverec.
+Qed.
+
+
+(*MOVE*)
+Definition lengthEq A :=
+  fix f (t:list A) n :=
+    match n,t with
+      0,nil => true
+    | (S n), _::t => f t n
+    | _,_ => false
+    end.
+Lemma lengthEq_spec A (t:list A) n:
+| t | =? n = lengthEq t n.
+Proof.
+  induction n in t|-*;destruct t;now cbn.
+Qed.
+Definition lengthEq_time k := k * 15 + 9.
+Instance term_lengthEq A `{registered A} : computableTime' (lengthEq (A:=A)) (fun l _ => (5, fun n _ => (lengthEq_time (min (length l) n),tt))).
+Proof.
+  extract. unfold lengthEq_time. solverec.
+Qed.
+
+
+Section concat.
+  Context X `{registered X}.
+
+  Fixpoint rev_concat acc (xs : list (list X)) :=
+    match xs with
+      [] => acc
+    | x::xs => rev_concat (rev_append x acc) xs
+    end.
+
+  Lemma rev_concat_rev xs acc:
+    rev (rev_concat acc xs) = rev acc ++ concat xs.
+  Proof.
+    induction xs in acc|-*. all:cbn. 2:rewrite IHxs,rev_append_rev. all:autorewrite with list in *. all:easy.
+  Qed.
+
+  Lemma rev_concat_length xs acc:
+    length (rev_concat acc xs) = length acc + length (concat xs).
+  Proof.
+    specialize (rev_concat_rev xs acc) as H1%(f_equal (@length _)).
+    autorewrite with list in H1. nia.
+  Qed.
+
   
+  Lemma _term_rev_concat :
+    { time : UpToC (fun l => sumn (map (@length _) l) + length l + 1) &
+             computableTime' (@rev_concat) (fun _ _ => (5,fun l _ => (time l,tt)))}.
+  Proof.      
+    evar (c1 : nat).
+    exists_UpToC (fun l => c1 * (sumn (map (@length _) l) + length l + 1) ).
+    { extract. recRel_prettify2.
+      all:cbn - [plus mult].
+      all:enough (c1>=20) by nia.
+      instantiate (c1:=20). all:subst c1;nia. 
+    }
+    smpl_upToC_solve.
+  Qed.
+  Global Instance term_rev_concat : computableTime' rev_concat _ := projT2 _term_rev_concat.
+
+  
+  Lemma _term_concat :
+    { time : UpToC (fun l => sumn (map (@length _) l) + length l + 1) &
+             computableTime' (@concat X) (fun l _ => (time l,tt))}.
+  Proof.
+    eexists_UpToC time. [time]: intros x.
+    eapply computableTimeExt with (x := fun l => rev (rev_concat [] l)).
+    -intros l;hnf. rewrite rev_concat_rev. easy.
+    -extract. solverec. unfold time. reflexivity.
+    -unfold time. setoid_rewrite rev_concat_length. setoid_rewrite length_concat. smpl_upToC_solve.
+  Qed.
+
+  Global Instance term_concat : computableTime' (@concat X) _ := projT2 _term_concat.
+End concat.
