theories/L/AbstractMachines/Computable/Shared.v
@@ -1,40 +1,29 @@
-From Undecidability.L Require Import L.
-From Undecidability.L.AbstractMachines Require Import Programs FunctionalDefinitions.
-From Undecidability.L.Datatypes Require Import LNat LProd Lists LOptions.
-From Undecidability.L.Tactics Require Import LTactics.
-Require Export List.
+From Undecidability.L Require Import L Tactics.LTactics.
+
+From Undecidability.L.AbstractMachines Require Import Programs FunctionalDefinitions AbstractHeapMachineDef.
+From Undecidability.L.Datatypes Require Import Lists LOptions LProd LTerm.
+
+From Undecidability.L Require Import Tactics.GenEncode.
 
 (** * Computability in L *)
-(** *** Encoding for Tokens *)
 
-Run TemplateProgram (tmGenEncode "token_enc" Tok).
-Hint Resolve token_enc_correct : Lrewrite.
+(** *** Encoding Heaps *)
+Import AbstractHeapMachineDef.
 
-Fixpoint jumpTarget_tr' l res P {struct P} : option (list Tok * list Tok) :=
-  match P with
-  | [] => None
-  | lamT :: P0 => jumpTarget_tr' (S l) (lamT::res) P0
-  | retT :: P0 => match l with
-                | 0 => Some (rev res, P0)
-                | S l0 => jumpTarget_tr' l0 (retT::res) P0
-                end
-  | t::P => jumpTarget_tr' l (t::res) P
-  end.
+Run TemplateProgram (tmGenEncode "heapEntry_enc" heapEntry).
+Hint Resolve heapEntry_enc_correct : Lrewrite.
 
-Definition jumpTarget_tr l res P := jumpTarget_tr' l (rev res) P.
-
-Lemma jumpTarget_tr_extEq : extEq  jumpTarget_tr jumpTarget.
-Proof.
-  intros l res P. unfold jumpTarget_tr. hnf.
-  induction P as [|[]]in res,l |-*. 5:destruct l.
-  all:cbn. all:try rewrite <- IHP. all:simpl_list;cbn. all:try congruence.
+Instance term_heapEntryC : computableTime' heapEntryC (fun _ _ => (1,fun _ _ => (1,tt))).
+extract constructor. solverec.
 Qed.
 
-Instance term_jump_target_tr' : computableTime jumpTarget_tr' (fun l _ => (5,fun res _ => (1,fun P _ => (length P * 36 +length res * 13 + 4,tt)))).
+(** *** Primitive functions with Heaps*)
+
+Instance term_get : computableTime' get (fun A _ => (1,fun n _ => (min n (length A)*15+16,tt))).
 extract. solverec.
 Qed.
 
-Instance term_jump_target : computableTime jumpTarget (fun l _ => (1,fun res _ => (1,fun P _ => (length P * 36 + length res * 26+ 21,tt)))).
-eapply computableTimeExt. now exact jumpTarget_tr_extEq. unfold jumpTarget_tr.
-extract. solverec. rewrite rev_length. Lia.lia.
+Import Datatypes.
+Instance put_get : computableTime' put (fun A _ => (1,fun _ _ => (length A * 27 + 22,tt))).
+extract. solverec.
 Qed.
