theories/L/AbstractMachines/LargestVar.v
@@ -1,0 +1,36 @@
+From Undecidability.L.Datatypes Require Import LProd LNat LTerm.
+
+Fixpoint largestVar (s:term) : nat :=
+  match s with
+    var n => n
+  | app s t => max (largestVar s) (largestVar t)
+  | lam s => largestVar s
+  end.
+
+
+Lemma largestVar_prod X Y `{Rx : registered X} {Ry : registered Y} (w:X*Y):
+  largestVar (enc w) = max (largestVar (enc (fst w))) (largestVar (enc (snd w))).
+Proof.
+  destruct w.
+  unfold enc. destruct Rx,Ry. cbn.  reflexivity.
+Qed.
+Lemma largestVar_nat (n:nat):
+  largestVar (enc n) <= 1.
+Proof.
+  unfold enc,registered_nat_enc.
+  induction n;cbn in *. all:Lia.lia.
+Qed.
+Lemma largestVar_term (s:term):
+  largestVar (enc s) <= 2.
+Proof.
+  unfold enc,registered_term_enc.
+  induction s;cbn -[max] in *.
+  1:rewrite largestVar_nat.
+  all:try Lia.lia.
+Qed.
+
+Lemma largestVar_size s :
+  largestVar s <= size s.
+Proof.
+  induction s;cbn;Lia.lia.
+Qed.
