theories/L/Computability/MuRec.v
@@ -119,3 +119,4 @@ End MuRecursor.
 
 Hint Resolve mu'_proc : LProc.
 Hint Resolve mu_proc : LProc.
+
