theories/L/Datatypes/LOptions.v
@@ -1,28 +1,30 @@
 From Undecidability.L Require Import Tactics.LTactics Datatypes.LBool Tactics.GenEncode.
+From Undecidability.L Require Import Functions.EqBool.
 Import L_Notations.
 
 (** ** Encoding of option type *)
 Section Fix_X.
   Variable X:Type.
-  Variable intX : registered X.
-  
+  Context {intX : registered X}.
+
+
   Run TemplateProgram (tmGenEncode "option_enc" (option X)).
   Hint Resolve option_enc_correct : Lrewrite.
-  
+
   (* now we must register the non-constant constructors*)
-  
-  Global Instance term_Some : computableTime (@Some X) (fun _ _ => (1,tt)).
+
+  Global Instance term_Some : computableTime' (@Some X) (fun _ _ => (1,tt)).
   Proof.
     extract constructor.
     solverec.
   Defined.
 
-  Lemma oenc_correct_some s (v : term) : lambda v -> enc s == ext (@Some X) v -> exists s', s = Some s' /\ v = enc s'.
-  Proof. 
+  Lemma oenc_correct_some (s: option X) (v : term) : lambda v -> enc s == ext (@Some X) v -> exists s', s = Some s' /\ v = enc s'.
+  Proof.
     intros lam_v H. unfold ext in H;cbn in H. unfold extT in H; cbn in H. redStep in H.
     apply unique_normal_forms in H;[|Lproc..]. destruct s;simpl in H.
     -injection H;eauto.
-    -discriminate H. 
+    -discriminate H.
   Qed.
        
 
@@ -46,7 +48,7 @@ Section option_eqb.
   Variable eqb : X -> X -> bool.
   Variable spec : forall x y, reflect (x = y) (eqb x y).
 
-  Definition option_eqb (A B : option X) := 
+  Definition option_eqb (A B : option X) :=
     match A,B with
     | None,None => true
     | Some x, Some y => eqb x y
@@ -65,11 +67,35 @@ Section int.
   Variable X:Type.
   Context {HX : registered X}.
 
-  Global Instance term_option_eqb : computableTime (@option_eqb X)
-                                                   (fun eqb eqbT => (1, fun a _ => (1,fun b _ => (match a,b with Some a, Some b => callTime2 eqbT a b + 10 | _,_ => 8 end,tt)))).
+  Global Instance term_option_eqb : computableTime' (@option_eqb X)
+                                                    (fun eqb eqbT => (1, fun a _ => (1,fun b _ => (match a,b with
+                                                                                            Some a, Some b => callTime2 eqbT a b + 10
+                                                                                          | _,_ => 8 end,tt)))). cbn.
   Proof.
     extract. solverec.
   Defined.
+
+  Global Instance eqbOption f `{eqbClass (X:=X) f}:
+    eqbClass (option_eqb f).
+  Proof.
+    intros ? ?. eapply option_eqb_spec. all:eauto using eqb_spec.
+  Qed.
+
+  Global Instance eqbComp_Option `{H:eqbCompT X (R:=HX)}:
+    eqbCompT (option X).
+  Proof.
+    evar (c:nat). exists c. unfold option_eqb. 
+    unfold enc;cbn.
+    change (eqb0) with (eqb (X:=X)).
+    extract. unfold eqb,eqbTime. fold (enc (X:=X)).
+    recRel_prettify2. easy.
+    [c]:exact (c__eqbComp X + 6).
+    all:unfold c. all:cbn iota beta delta [option_enc].
+    all:  change ((match HX with
+           | @mk_registered _ enc _ _ => enc
+           end)) with (enc (X:=X)).
+    all:cbn [size]. all: nia.
+  Qed.
 
 End int.
 
@@ -78,4 +104,16 @@ Definition isSome {T} (u : option T) := match u with Some _ => true | _ => false
 Instance term_isSome {T} `{registered T} : computable (@isSome T).
 Proof.
   extract.
+Qed.
+
+
+Lemma size_option X `{registered X} (l:option X):
+  size (enc l) = match l with Some x => size (enc x) + 5 | _ => 3 end.
+Proof.
+  change (enc l) with (option_enc l).
+  destruct l. all:cbn [option_enc map sumn size].
+  change ((match H with
+           | @mk_registered _ enc _ _ => enc
+           end x)) with (enc x).
+  all:lia. 
 Qed.
