theories/L/Datatypes/LTerm.v
@@ -7,17 +7,33 @@ Run TemplateProgram (tmGenEncode "term_enc" term).
 Hint Resolve term_enc_correct : Lrewrite.
   
 (* register the non-constant constructors *)
-Instance term_var : computableTime var (fun n _ => (1, tt)).
+Instance term_var : computableTime' var (fun n _ => (1, tt)).
 Proof.
   extract constructor. solverec.
 Defined.
 
-Instance term_app : computableTime L.app (fun s1 _ => (1, (fun s2 _ => (1, tt)))).
+Instance term_app : computableTime' L.app (fun s1 _ => (1, (fun s2 _ => (1, tt)))).
 Proof.
   extract constructor. solverec.
 Defined.
 
-Instance term_lam : computableTime lam (fun s _ => (1, tt)).
+Instance term_lam : computableTime' lam (fun s _ => (1, tt)).
 Proof.
   extract constructor. solverec.
 Defined.
+
+
+Lemma size_term_enc (s:term) :
+  size (enc s) <= size s *11.
+Proof.
+  induction s;cbv [enc registered_term_enc] in *. all:cbn [size term_enc] in *.
+  rewrite size_nat_enc. all:solverec.
+Qed.
+
+
+Lemma size_term_enc_r (s:term) :
+  size s <= size (enc s).
+Proof.
+  induction s;cbv [enc registered_term_enc] in *. all:cbn [size term_enc] in *.
+  rewrite <- size_nat_enc_r. all:solverec.
+Qed.
