theories/L/Functions/FinTypeLookup.v
@@ -1,0 +1,96 @@
+From Undecidability.L.Tactics Require Import LTactics.
+From Undecidability.L.Datatypes Require Import LFinType LBool LProd Lists.
+From Undecidability.L.Functions Require Import EqBool.
+
+Section Lookup.
+  Variable X Y : Type.
+  Context {eqbX : X -> X -> bool}.
+  Context `{eqbClass X eqbX}.
+
+  Fixpoint lookup (x:X) (A:list (X*Y)) d: Y :=
+    match A with
+      [] => d
+    | (key,Lproc)::A =>
+      if eqb x key then Lproc else lookup x A d
+    end.
+
+  Context `{registered X} `{@eqbCompT X _ eqbX _}.
+
+  Definition lookupTime (x:nat) (l:list (X*Y)):=
+    fold_right (fun '(a,b) res => eqbTime (X:=X) x (size (enc (a:X))) + res +24) 4 l.
+
+  Global Instance term_lookup `{registered Y}:
+    computableTime' (lookup) (fun x _ => (5, fun l _ => (1, fun d _ => (lookupTime (size (enc x)) l,tt)))).
+  unfold lookup. unfold eqb.
+  extract. unfold lookupTime. solverec.
+  Qed.
+
+  Lemma lookupTime_leq x (l:list (X*Y)):
+    lookupTime x l <= length l * (x* c__eqbComp X + 24) + 4.
+  Proof.
+    induction l as [ | [a b] l].
+    -cbn. omega.
+    -unfold lookupTime. cbn [fold_right]. fold (lookupTime x l).
+     rewrite eqbTime_le_l.
+     setoid_rewrite IHl. cbn [length].
+     ring_simplify. unfold eqb. omega.
+  Qed.
+
+End Lookup.
+
+Section funTable.
+
+  Variable X : finType.
+  Variable Y : Type.
+  Variable f : X -> Y.
+
+  Definition funTable :=
+    map (fun x => (x,f x)) (elem X).
+
+
+  Variable (eqbX : X -> X -> bool).
+  Context `{eqbClass X eqbX}.
+
+  Lemma lookup_funTable x d:
+    lookup x funTable d = f x.
+  Proof.
+    unfold funTable.
+    specialize (elem_spec x).
+    generalize (elem X) as l.
+    induction l;cbn;intros Hel.
+    -tauto.
+    -destruct (eqb_spec x a).
+     +congruence.
+     +destruct Hel. 1:congruence.
+      eauto.
+  Qed.
+  
+End funTable.
+
+Lemma lookup_sound' (A: Type) (B: Type) eqbA `{eqbClass (X:=A) eqbA} (L : list (prod A B)) a b def :
+  (forall a' b1 b2, (a',b1) el L -> (a',b2) el L -> b1=b2) -> ( (a,b) el L \/ ((forall b', ~ (a,b') el L) /\ b = def) ) -> lookup a L def = b.
+Proof.
+  intros H1 H2.
+  induction L as [ |[a' b'] L]. now intuition.
+  cbn.
+  destruct (eqb_spec a a').
+  -subst a. destruct H2.
+   2:now exfalso.
+   eapply H1. all:easy.
+  -apply IHL. all:intros.
+   +eapply H1. all:eauto.
+   +destruct H2 as [[]|]. all:easy.
+Qed.
+
+Lemma lookup_complete (A: Type) (B: Type) eqbA `{eqbClass (X:=A) eqbA} (L : list (prod A B)) a def :
+  {(a,lookup a L def) el L } + {~(exists b, (a,b) el L) /\ lookup a L def  = def}.
+Proof.
+  induction L as [ |[a' b'] L].
+  -cbn. right. firstorder.
+  -cbn.  destruct (eqb_spec a a').
+   1:{ do 2 left. congruence. }
+   destruct IHL as [|[? eq]];[left|right].
+   +eauto.
+   +split. 2:easy.
+    now intros (?&[]). 
+Qed.
