theories/L/Tactics/mixedTactics.v
@@ -1,4 +1,4 @@
-Require Import PslBase.Base.
+Require Import PslBase.Base Lia Ring.
 
 Tactic Notation "destruct" "_":= 
   match goal with
@@ -22,3 +22,7 @@ Ltac trace :=
   match goal with
     |- ?G => idtac "Trace:";idtac G
   end.
+
+Ltac leq_crossout :=
+       try zify;try apply Zle_0_minus_le; ring_simplify;
+       repeat eapply Z.add_nonneg_nonneg;try now (repeat eapply Z.mul_nonneg_nonneg;easy).
